<?xml version="1.0"?>
<rdf:RDF xmlns="https://w3id.org/framester/conceptnet/schema#"
     xml:base="https://w3id.org/framester/conceptnet/schema"
     xmlns:dc="http://purl.org/dc/elements/1.1/"
     xmlns:owl="http://www.w3.org/2002/07/owl#"
     xmlns:rdf="http://www.w3.org/1999/02/22-rdf-syntax-ns#"
     xmlns:xml="http://www.w3.org/XML/1998/namespace"
     xmlns:xsd="http://www.w3.org/2001/XMLSchema#"
     xmlns:rdfs="http://www.w3.org/2000/01/rdf-schema#"
     xmlns:data-view="http://www.w3.org/2003/g/data-view#">
    <owl:Ontology rdf:about="https://w3id.org/framester/conceptnet/schema">
        <owl:versionIRI rdf:resource="https://w3id.org/framester/conceptnet/0.0.1"/>
        <owl:imports rdf:resource="https://w3id.org/framester/metadata/schema/0.0.1"/>
        <dc:title xml:lang="en">Framester&apos;s Ontology of ConceptNet</dc:title>
        <rdfs:comment xml:lang="en">This ontology formalizes the schema used in Framester for structuring knowledge from ConceptNet.



This work includes data from ConceptNet 5, which was compiled by the
Commonsense Computing Initiative. ConceptNet 5 is freely available under
the Creative Commons Attribution-ShareAlike license (CC BY SA 3.0) from
http://conceptnet.io.

The included data was created by contributors to Commonsense Computing
projects, contributors to Wikimedia projects, DBPedia, OpenCyc, Games
with a Purpose, Princeton University&apos;s WordNet, Francis Bond&apos;s Open
Multilingual WordNet, and Jim Breen&apos;s JMDict.</rdfs:comment>
        <owl:versionInfo xml:lang="en">0.0.1</owl:versionInfo>
    </owl:Ontology>
    


    <!-- 
    ///////////////////////////////////////////////////////////////////////////////////////
    //
    // Object Properties
    //
    ///////////////////////////////////////////////////////////////////////////////////////
     -->

    


    <!-- https://w3id.org/framester/conceptnet/schema/sourceDataset -->

    <owl:ObjectProperty rdf:about="https://w3id.org/framester/conceptnet/schema/sourceDataset">
        <rdfs:comment xml:lang="en">The ConceptNet&apos;s source dataset where the assertion comes from.</rdfs:comment>
        <rdfs:label xml:lang="en">source dataset</rdfs:label>
    </owl:ObjectProperty>
    


    <!-- 
    ///////////////////////////////////////////////////////////////////////////////////////
    //
    // Data properties
    //
    ///////////////////////////////////////////////////////////////////////////////////////
     -->

    


    <!-- https://w3id.org/framester/conceptnet/schema/conceptNetIdentifier -->

    <owl:DatatypeProperty rdf:about="https://w3id.org/framester/conceptnet/schema/conceptNetIdentifier">
        <rdfs:comment xml:lang="en">The identifier of a ConceptNet&apos;s concept, relation or assertion.</rdfs:comment>
        <rdfs:label xml:lang="en">ConceptNet Identifier</rdfs:label>
    </owl:DatatypeProperty>
    


    <!-- https://w3id.org/framester/conceptnet/schema/conceptNetWeight -->

    <owl:DatatypeProperty rdf:about="https://w3id.org/framester/conceptnet/schema/conceptNetWeight">
        <rdfs:subPropertyOf rdf:resource="https://w3id.org/framester/metadata/schema/confidence"/>
        <rdf:type rdf:resource="http://www.w3.org/2002/07/owl#FunctionalProperty"/>
        <rdfs:domain rdf:resource="https://w3id.org/framester/conceptnet/schema/Assertion"/>
        <rdfs:comment xml:lang="en">The weight of a ConceptNet&apos;s assertion.</rdfs:comment>
        <rdfs:label>weight</rdfs:label>
    </owl:DatatypeProperty>
    


    <!-- 
    ///////////////////////////////////////////////////////////////////////////////////////
    //
    // Classes
    //
    ///////////////////////////////////////////////////////////////////////////////////////
     -->

    


    <!-- https://w3id.org/framester/conceptnet/schema/Assertion -->

    <owl:Class rdf:about="https://w3id.org/framester/conceptnet/schema/Assertion">
        <rdfs:subClassOf>
            <owl:Restriction>
                <owl:onProperty rdf:resource="https://w3id.org/framester/conceptnet/schema/sourceDataset"/>
                <owl:allValuesFrom rdf:resource="http://www.w3.org/2002/07/owl#Thing"/>
            </owl:Restriction>
        </rdfs:subClassOf>
        <rdfs:comment xml:lang="en">An edge, or assertion, is a unit of knowledge in ConceptNet. It tells us a particular relation between natural-language terms, according to a particular source.</rdfs:comment>
        <rdfs:label xml:lang="en">Assertion</rdfs:label>
    </owl:Class>
    


    <!-- https://w3id.org/framester/conceptnet/schema/Concept -->

    <owl:Class rdf:about="https://w3id.org/framester/conceptnet/schema/Concept">
        <rdfs:label xml:lang="en">Concept</rdfs:label>
    </owl:Class>
    


    <!-- https://w3id.org/framester/conceptnet/schema/Relation -->

    <owl:Class rdf:about="https://w3id.org/framester/conceptnet/schema/Relation">
        <rdfs:comment xml:lang="en">A relation between two ConceptNet&apos;s concepts.</rdfs:comment>
        <rdfs:label xml:lang="en">Relation</rdfs:label>
    </owl:Class>
</rdf:RDF>



<!-- Generated by the OWL API (version 4.5.9.2019-02-01T07:24:44Z) https://github.com/owlcs/owlapi -->

